Good progress when compilation/instrumentation

io/ILang.CompileTo.TLang.fst
@@ -17,14 +17,14 @@ open TC.Checkable
 class compilable (t:Type) (pi:monitorable_prop) = {
   c_t_ilang : ilang t pi;
   comp_type : Type;
-  c_comp_type : tlang comp_type;
+  c_comp_type : mlang comp_type;
   compile: t -> comp_type
   // CC theorem?
   // c_compile: squash (forall (wS:t). theta (reify (compile wS)) `hist_ord` theta (reify wS)) 
 }
 
 class instrumentable (t:Type) (pi:monitorable_prop) = {
-  cc_t_ilang : ilang t pi;
+  cc_t_ilang : mlang t pi;
   inst_type : Type;
   c_inst_type : tlang inst_type;
   c_pi:squash (forall h cmd arg. pi cmd arg h ==> io_pre cmd arg h);
@@ -58,7 +58,7 @@ instance compile_ilang_base (t1:Type u#0) (t2:Type u#0) pi {| d1:instrumentable 
     (** TODO: I have no idea what happens with the raise_t of the result. 
         I suppose for now it does not care. There is a Universe.downgrade_val in the theta and I suppose there will be another
         downgrade_val when interpreting the tree. **)
-    let dm : dm_iio (resexn d2.comp_type) (trivial_hist ()) = Decorated (fun h lt -> b2t (enforced_locally pi h lt)) x' Return in
+    let dm : dm_iio (resexn d2.comp_type) trivial_hist = Decorated (fun h lt -> b2t (enforced_locally pi h lt)) x' Return in
     IIOwp?.reflect dm
   );
 }
@@ -88,37 +88,131 @@ assume val dynamic_cmd :
          | Inr Contract_failure -> ~(d1.check2 arg h) /\ lt == []
          | _ -> d1.check2 arg h /\ lt == [convert_call_to_event cmd arg r]) ==> p lt r))
 
+let t () : Tac unit = l_to_r [`Common.rev_nil;`List.Tot.Properties.append_nil_l;`List.Tot.Properties.append_l_nil]; trefl ()
+
+[@@ (postprocess_with t)]
 let run_m
   (pi:monitorable_prop)
-  (tree : dm_iio 'b (fun p h -> forall lt r. enforced_locally pi h lt ==> p lt r)) :
-  IIOpi 'b pi =
-  let tree : dm_iio 'b (fun p h -> forall (r: 'b) (lt: trace). enforced_locally pi h lt ==> p lt r) = tree in
-  IIOwp?.reflect tree
+  (m : iio (Universe.raise_t 'b))
+  dec
+  k
+  p
+  (h:trace)
+  (_:squash (dm_iio_theta (Decorated dec m k) p h))
+  (_:squash (forall h lt. dec h lt ==> enforced_locally pi h lt))
+  (_:squash (dm_iio_theta m (fun lt r -> enforced_locally pi h lt) h)) :
+  IIO 
+    (Universe.raise_t 'b * trace * _)
+    (requires (fun h' -> h == h'))
+    (ensures (fun h res lt ->
+      Mktuple3?._2 res == apply_changes h lt /\
+      dm_iio_theta (k (Universe.downgrade_val (Mktuple3?._1 res))) (Mktuple3?._3 res) (Mktuple3?._2 res) /\
+      enforced_locally pi h lt)) =
+  let theM : unit -> IIOwp _ (fun p h' -> h == h' /\ (forall lt r. enforced_locally pi h lt ==> p lt r)) = (fun () -> IIOwp?.reflect m) in
+  let r = theM () in 
+  Classical.forall_intro (lemma_suffixOf_append h);
+  let lt = IIO.CompileTo.ILang.extract_local_trace h pi in
+  let p' = hist_post_shift p lt in
+  let h' = apply_changes h lt in
+  let z' = k (Universe.downgrade_val r) in
+  assume (dm_iio_theta z' p' h');
+  (r, h', p')
+
+let rec inside_respects_pi
+  (tree : iio (resexn 'a))
+  (pi : monitorable_prop) : Type0 =
+  match tree with
+  | Return _ -> True
+  | PartialCall pre k ->
+      pre ==> (inside_respects_pi (k ()) pi)
+  | Call cmd arg k ->
+      forall res. inside_respects_pi (k res) pi
+  | Decorated dec m k ->
+      (forall h lt. dec h lt ==> enforced_locally pi h lt) /\
+      (forall res. inside_respects_pi (k res) pi)
+
+(**
+let lemma_theta_decorated_rhs dec m k p h :
+  Lemma
+    (requires (dm_iio_theta (Decorated dec m k) p h))
+    (ensures (forall lt res. dm_iio_theta (k res) p h))
+**)
+(**    calc (==>) {
+      dm_iio_theta (Decorated d m k) p h;
+      ==> { _ by (
+            binder_retype (nth_binder (-1));
+            norm [delta_only [`%dm_iio_theta;`%DMFree.theta]; zeta];
+            trefl ();
+            norm [delta_only [`%dm_iio_theta]];
+            assumption ()) }
+      hist_bind
+             (fun p h -> dm_iio_theta m (fun lt r -> d h lt /\ p lt r) h)
+             (fun r -> dm_iio_theta (k (Universe.downgrade_val r))) p h;
+      ==> {}
+      hist_bind
+             (fun p h -> dm_iio_theta m (fun lt r -> enforced_locally pi h lt /\ p lt r) h)
+             (fun r -> dm_iio_theta (k (Universe.downgrade_val r))) p h;
+      ==> { _ by (binder_retype (nth_binder (-1));
+                  norm [delta_only [`%hist_bind;`%hist_post_bind]]; trefl (); assumption ()) }
+      dm_iio_theta m
+        (fun lt r ->
+          enforced_locally pi h lt /\
+          dm_iio_theta (k (Universe.downgrade_val r))
+            (hist_post_shift p lt)
+            (List.Tot.Base.rev lt @ h)) h;
+      ==> {}
+      dm_iio_theta m
+        (fun lt r ->
+          dm_iio_theta (k (Universe.downgrade_val r))
+            (hist_post_shift p lt)
+            (List.Tot.Base.rev lt @ h)) h;
+    }; **)
+
+open FStar.List.Tot
+   
+let lemma_smt_pat (pi:monitorable_prop) (h lt1 lt2:trace) :
+  Lemma (requires (
+    enforced_locally pi h lt1 /\
+    enforced_locally pi (apply_changes h lt1) lt2))
+    (ensures (
+    enforced_locally pi h (lt1 @ lt2))) [SMTPat (enforced_locally pi h (lt1@lt2))] = admit ()
 
 let rec _instrument
-  (tree : dm_iio (resexn 'a) (trivial_hist ()))
-  (pi    : monitorable_prop)
+  (tree : iio (resexn 'a))
+  (p    : hist_post (resexn 'a))
+  (h    : trace)
+  (_    : squash (dm_iio_theta tree p h))
+  (pi   : monitorable_prop)
+  (_:squash (inside_respects_pi tree pi))
   (c_pi:squash (forall h cmd arg. pi cmd arg h ==> io_pre cmd arg h)) :
-  IIOpi (resexn 'a) pi =
+  IIOwp (resexn 'a) (fun p h' -> h == h' /\ (forall lt r. enforced_locally pi h lt ==> p lt r)) by (
+    l_to_r [`Common.rev_nil; `List.Tot.Properties.append_nil_l; `List.Tot.Properties.append_l_nil]
+  ) =
   match tree with
-  | Return r -> r
+  | Decorated d #b m k ->
+    let res = run_m pi m d k p h () () () in
+    let r = Mktuple3?._1 res in
+    let h' = Mktuple3?._2 res in
+    let p' = Mktuple3?._3 res in
+    let z' : iio (resexn 'a) = k (FStar.Universe.downgrade_val r) in
+    let proof1 : squash (dm_iio_theta z' p' h') = () in
+    let proof2 : squash (inside_respects_pi z' pi) = () in
+    _instrument z' p' h' proof1 pi proof2 c_pi
   | Call GetTrace argz fnc -> Inr Contract_failure
   | PartialCall pre fnc -> Inr Contract_failure
-  | Decorated d #b m k ->
-      assume (forall h. dm_iio_theta m (fun lt r -> enforced_locally pi h lt) h);
-      let r : b = FStar.Universe.downgrade_val (run_m pi m) in
-      let z' : iio (resexn 'a) = k r in
-      assume (trivial_hist () `hist_ord` dm_iio_theta z');
-      admit ();
-      _instrument z' pi c_pi
+  | Return r -> r
   | Call cmd argz fnc -> begin
     let d : checkable2 (io_pre cmd) = (
       implies_is_checkable2 (io_sig.args cmd) trace (pi cmd) (io_pre cmd) c_pi) in
     (** Check if the runtime check failed, and if yes, return the error **)
     let rez = dynamic_cmd cmd d argz in
     let z' : iio (resexn 'a) = fnc rez in
-    assume (trivial_hist () `hist_ord` dm_iio_theta z');
-    _instrument z' pi c_pi
+
+    let p' : hist_post (resexn 'a) = hist_post_shift p [convert_call_to_event cmd argz rez] in
+    let h' = apply_changes h [convert_call_to_event cmd argz rez] in
+    let proof1 : squash (dm_iio_theta z' p' h') = () in
+    let proof2 : squash (inside_respects_pi z' pi) = () in
+    _instrument z' p' h' proof1 pi proof2 c_pi
   end
 
 instance instrumentable_arrow t1 t2 pi {| d1:compilable t1 pi |} {| d2:instrumentable t2 pi |} : instrumentable (t1 -> IIOpi (resexn t2) pi) pi = {
@@ -127,8 +221,11 @@ instance instrumentable_arrow t1 t2 pi {| d1:compilable t1 pi |} {| d2:instrumen
   c_inst_type = tlang_arrow d1.comp_type d2.inst_type #d1.c_comp_type #d2.c_inst_type;
   c_pi = d2.c_pi;
   instrument = (fun (f:d1.comp_type -> MIIO (resexn d2.inst_type)) (x:t1) -> 
-    let tree : dm_iio (resexn d2.inst_type) (trivial_hist ()) = reify (f (compile x)) in
-    let r  : resexn d2.inst_type = _instrument #d2.inst_type tree pi d2.c_pi in 
+    let tree : dm_iio (resexn d2.inst_type) trivial_hist = reify (f (compile x)) in
+    let p = fun _ _ -> True in
+    let h = get_trace () in
+    assume (inside_respects_pi tree pi);
+    let r  : resexn d2.inst_type = _instrument #d2.inst_type tree p h () pi () d2.c_pi in 
     instrument #_ #pi #(instrumentable_resexn pi t2 #d2) r 
   )
 }
